Hashmap/HashMap.lean
@@ -29,37 +29,87 @@ theorem update_get [BEq α] {b : Buckets α β} {i : Fin b.1.size} {l : AssocLis
   simp [update]
   rw [Array.get_set]
 
-structure BucketWFAt [BEq α] [Hashable α] (l : AssocListMap α β)
-    (size i : Nat) : Prop where
-  hash_valid [LawfulHashable α] : ∀ a, l.contains a → (hash a % size).toNat = i
+private def mkIdx {sz : Nat} (hash : UInt64) (h : sz.isPowerOfTwo) : { u : USize // u.toNat < sz } :=
+  -- TODO: avoid `if` in the reference implementation
+  let u := hash.toUSize &&& (sz.toUSize - 1)
+  if h' : u.toNat < sz then
+    ⟨u, h'⟩
+  else
+    ⟨0, by simp [USize.toNat, OfNat.ofNat, USize.ofNat, Fin.ofNat']; apply Nat.pos_of_isPowerOfTwo h⟩
 
-theorem BucketWFAt_nil [BEq α] [Hashable α] {size i : Nat} :
-    BucketWFAt (AssocListMap.nil : AssocListMap α β) size i where
+def mkIdx' {sz : Nat} (hash : UInt64) (h : sz.isPowerOfTwo) : Fin sz :=
+  let i := mkIdx hash h; ⟨i.1.toNat, i.2⟩
+
+structure BucketWFAt [BEq α] [Hashable α] (l : AssocListMap α β)
+    {size : Nat} (h : size.isPowerOfTwo) (i : Nat) : Prop where
+  hash_valid [LawfulHashable α] : ∀ a, l.contains a → (mkIdx (hash a) h).1.toNat = i
+
+theorem BucketWFAt_nil [BEq α] [Hashable α] {size : Nat} (h : size.isPowerOfTwo) {i : Nat} :
+    BucketWFAt (AssocListMap.nil : AssocListMap α β) h i where
   hash_valid a h := by simp at h
 
-theorem BucketWFAt_erase [BEq α] [EquivBEq α] [Hashable α] {l : AssocListMap α β} {k : α} {size i : Nat} :
-    BucketWFAt l size i → BucketWFAt (l.erase k) size i :=
+theorem BucketWFAt_erase [BEq α] [EquivBEq α] [Hashable α] {l : AssocListMap α β} {k : α} {size : Nat}
+    (h : size.isPowerOfTwo) {i : Nat} :
+    BucketWFAt l h i → BucketWFAt (l.erase k) h i :=
   fun ⟨h⟩ => ⟨fun a h' => h a <| l.contains_of_contains_erase h'⟩
 
-theorem BucketWFAt_insert [BEq α] [EquivBEq α] [Hashable α] {l : AssocListMap α β} {k : α} {v : β k} {size i : Nat}
-    (h : (hash k % size).toNat = i) : BucketWFAt l size i → BucketWFAt (l.insert k v) size i := by
-  refine fun ⟨h⟩ => ⟨fun a h' => ?_⟩
-  rw [l.contains_insert, Bool.or_eq_true] at h'
-  rcases h' with (h'|h')
-  · rwa [← hash_eq_of_beq h']
-  · exact h _ h'
+theorem BucketWFAt_insert [BEq α] [EquivBEq α] [Hashable α] {l : AssocListMap α β} {k : α} {v : β k} {size : Nat}
+    (h' : size.isPowerOfTwo) {i : Nat}
+    (h : (mkIdx (hash k) h').1.toNat = i) : BucketWFAt l h' i → BucketWFAt (l.insert k v) h' i := by
+  refine fun ⟨h₁⟩ => ⟨fun a h'' => ?_⟩
+  rw [l.contains_insert, Bool.or_eq_true] at h''
+  rcases h'' with (h''|h'')
+  · rwa [← hash_eq_of_beq h'']
+  · exact h₁ _ h''
 
 structure WF [BEq α] [Hashable α] [LawfulHashable α] (b : Buckets α β) : Prop where
-  bucket_wf : ∀ (i : Fin b.1.size), BucketWFAt b.1[i] b.1.size i
+  bucket_wf : ∀ (i : Fin b.1.size), BucketWFAt b.1[i] b.2 i
 
 theorem WF_update [BEq α] [Hashable α] [LawfulHashable α] {b : Buckets α β} {i : Fin b.1.size}
-    {l : AssocListMap α β} : b.WF → BucketWFAt l b.1.size i → (b.update i l).WF := by
+    {l : AssocListMap α β} : b.WF → BucketWFAt l b.2 i → (b.update i l).WF := by
   refine fun ⟨h₁⟩ h₂ => ⟨fun j => ?_⟩
   rw [update_get]
   by_cases h' : i.1 = j
   · simpa [h'] using h₂
   · simp [h']
     apply h₁ (Fin.cast (by simp) j)
+
+-- def bucketFor [BEq α] [Hashable α] (b : Buckets α β) (k : α) : AssocListMap α β :=
+--   b.1[mkIdx' (hash k) b.2]
+
+def contains [BEq α] [Hashable α] (b : Buckets α β) (k : α) : Bool :=
+  b.1[mkIdx' (hash k) b.2].contains k
+
+def cons [BEq α] [Hashable α] (b : Buckets α β) (k : α) (v : β k) (h : b.contains k = false) : Buckets α β :=
+  let idx := mkIdx' (hash k) b.2;
+  b.update idx (b.1[idx].cons k v h)
+
+@[simp]
+theorem contains_cons [BEq α] [Hashable α] (b : Buckets α β) {k a : α} {v : β k} {h : b.contains k = false} :
+    (b.cons k v h).contains a = (k == a || b.contains a) := sorry
+
+structure Consable [BEq α] [Hashable α] (b : Buckets α β) (l : AssocListMap α β) : Prop where
+  contains : ∀ a, l.contains a → b.contains a = false
+
+theorem Consable.cons_out [BEq α] [EquivBEq α] [Hashable α] {b : Buckets α β} {l : AssocListMap α β} {k : α}
+    {v : β k} {h : l.contains k = false} : Consable b (l.cons k v h) → b.contains k = false
+  | ⟨h⟩ => h _ (by simp)
+
+theorem consable_nil [BEq α] [Hashable α] {b : Buckets α β} : Consable b AssocListMap.nil where
+  contains := by simp
+
+theorem consable_cons [BEq α] [EquivBEq α] [Hashable α] {b : Buckets α β}
+    {l : AssocListMap α β} {k : α} {v : β k} {h : l.contains k = false}
+      (hb : Consable b (l.cons k v h)) : Consable (b.cons k v hb.cons_out) l where
+  contains a ha := by
+    simp [Bool.or_eq_false_iff]
+    refine ⟨?_, ?_⟩
+    · -- Contradiction using h and ha
+      sorry
+    · apply hb.contains
+      simpa using Or.inr ha
+
+-- def addAll (b : Buckets α β) (l : AssocListMap α β) (h : ∀ a, l.contains a →
 
 end Buckets
 
